src/crypto/poly1305/x64/X64.Poly1305.Math_i.fsti
@@ -82,10 +82,11 @@ val lemma_poly_multiply : n:int -> p:int -> r:int -> h:int -> r0:int -> r1:int -
 	(ensures (h * r) % p == hh % p)
 
 // p used to be a refinement to p > 0 and h a nat.
-val lemma_poly_reduce : n:int -> p:pos -> h:nat -> h2:nat -> h10:int -> c:int -> hh:int -> Lemma
+val lemma_poly_reduce : n:int -> p:int -> h:int -> h2:int -> h10:int -> c:int -> hh:int -> Lemma
   (requires
+    p > 0 /\
     n * n > 0 /\
-    h2 >= 0 /\  // TODO: Shouldn't need to add this
+    h >= 0 /\ h2 >= 0 /\  // TODO: Shouldn't need to add this
     4 * (n * n) == p + 5 /\
     h2 == h / (n * n) /\
     h10 == h % (n * n) /\
@@ -108,12 +109,12 @@ val lemma_poly_bits64 : u:unit -> Lemma
     (forall (x:nat64) . {:pattern (logand64 x 0x0ffffffc0ffffffc)} (logand64 x 0x0ffffffc0ffffffc) % 4 == 0) /\
     (forall (x:nat64)  (y:nat64) . (logand64 x y) == (logand64 y x)))
 
-val lemma_mul_strict_upper_bound : x:nat -> x_bound:int -> y:nat -> y_bound:int -> Lemma
+val lemma_mul_strict_upper_bound : x:int -> x_bound:int -> y:int -> y_bound:int -> Lemma
   (requires 
-    x < x_bound /\
-    y < y_bound)
+    0 <= x /\ x < x_bound /\
+    0 <= y /\ y < y_bound)
   (ensures x * y < x_bound * y_bound)
-    
+
 val lemma_bytes_shift_power2 : y:nat64 -> Lemma
   (requires y < 8)
   (ensures 
